№1
$xy \lor (x\neg y \lor \neg xy) = xy \lor x \neg y \lor \neg x y = x \lor \neg xy = x \lor y$
$xy \to x = \neg(xy) \lor x = \neg x \lor \neg y \lor x = 1$
$f = (\neg x \to z) \to \neg(\neg y \to \neg x) = (x \lor z) \to (\neg y \land x) = \neg x \land \neg z \lor \neg y \land x$
СДНФ: $\neg x \neg z y \lor \neg x \neg z \neg y \lor x \neg y z \lor z \neg y \neg z$
$f = x(yz \to xy) = x(\neg(y \land z) \lor x \land y) = x \land \neg y \lor x \land \neg z \lor x \land y = x(\neg y \lor \neg z \lor y)$
СКНФ: $(\neg x \lor \neg y \lor \neg z) \land (\neg x \lor \neg y \lor z) \land (\neg x \lor y \lor \neg z) \land (\neg x \lor y \lor z) \land (x \lor y \lor z) \land (x \lor \neg y \lor z)$


1. Сохраняет 0 $f(0,\dots, 0) = 0$
2. Сохраняет 1 $f(1,\dots, 1) = 1$
3. Монотонная
4. Самодвойственная
5. Линейная

№2
Линейная $f=(01001100)$

#0
1. no
2. yes
3. yes
4. no
5. $f = 1$

#1
1. yes
2. no
3. yes
4. $f(\neg0) = f(1) = 0 = f(0)$
5. $f = 0$

#$\land$
1. yes
2. no
3. no
4. $f(\neg x ; \neg y) = \neg f(x;y)$
5. $f = xy$

#$\lor$
1. yes
2. yes
3. yes
4. $f(\neg x \lor \neg y) = \neg f(x \lor y)$
5. $f = x + y + xy$

#$\neg$
1. no
2. no
3. no
4. $f(\neg x) = \neg f(x)$
5. $f = \neg x$

#$\to$
1. no
2. yes
3. no
4. $f(\neg x; \neg y) = \neg f(x;y)$
5. $f = x+xy+1$

#$\downarrow$
1. no
2. no
3. no
4. $f(\neg x;\neg y) = \neg f(x;y)$
5. $f = y + x++xy$

#$\leftrightarrow$
1. no
2. yes
3. no
4. $f(\neg x \leftrightarrow \neg y) = \neg f(x \leftrightarrow y)$
5. $f = 1 + x + y$

#$|$
1. no
2. no
3. no
4. $f(\neg x | \neg y) = \neg f(x | y)$
5. $f = 1+xy$


№3
#$\neg$
1. no
2. no
3. no
4. yes
5. no

#$\cap$
1. yes
2. yes
3. yes
4. no
5. no

{$\neg, \land$} - базис


№4
1) $f(11110001)$
		x y z f
		0 0 0 1
		0 0 1 1
		0 1 0 1
		0 1 1 1
		1 0 0 0
		1 0 1 0
		1 1 0 0
		1 1 1 1
	$СДНФ: f:(\neg x \land \neg y \land \neg z) \lor (\neg x \land \neg y \land z) \lor (\neg x \land y \land z) \lor (x \land y \land z)$
	СКНФ: $f: (\neg x \lor y \lor z) \land (\neg x \lor y \lor \neg z) \land (\neg x \lor \neg y \lor z)$

2) $f(00010101)$
		x y z f
		0 0 0 0
		0 0 1 0
		0 1 0 0
		0 1 1 1
		1 0 0 0
		1 0 1 1
		1 1 0 0
		1 1 1 1
	$СДНФ: f:(\neg xyz \lor xy\neg z \lor xyz)$
	СКНФ: $f: (x \lor y \lor z) \land (x \lor y \lor \neg z) \land (x \lor \neg y \lor z) \land (\neg x \lor y \lor z) \land (\neg x \lor y \lor \neg z)$


№5
1) f=(--0-01--) f∈M
		x y z f
		0 0 0 0
		0 0 1 0
		0 1 0 0
		0 1 1 0
		1 0 0 0
		1 0 1 1
		1 1 0 1
		1 1 1 1
	f=(00000111)

2) g=(--0-01--) g∈L
		x y z f
		0 0 0 
		0 0 1 
		0 1 0 
		0 1 1 1
		1 0 0 
		1 0 1 0
		1 1 0 1
		1 1 1 0
	g=(---1-010)

3) h=(1-10--1-) h∈S
		x y z f
		0 0 0 1
		0 0 1 0
		0 1 0 1
		0 1 1 0
		1 0 0 1
		1 0 1 0
		1 1 0 1
		1 1 1 0
	h=(10101010)


№6
f=(10100001)
g=(00111100)
{f ; g}
	x y z f g
	0 0 0 1 0
	0 0 1 0 0
	0 1 0 1 1
	0 1 1 0 1
	1 0 0 0 1
	1 0 1 0 1
	1 1 0 0 0
	1 1 1 1 0