$(x-2)^7=C_{7}^0x^7(-2)^0+C_{7}^1x^6(-2)^1+C_{7}^2x^5(-2)^2+C_{7}^3x^4(-2)^3+C_{7}^4x^3(-2)^4+C_{7}^5x^2(-2)^5+$
$+C_{7}^6x^1(-2)^6+C_{7}^7x^0(-2)^7=x^7-14x^6+84x^5-280x^4+560x^3-672x^2+448x-128$

$\left( \frac{1}{\sqrt{ 3x }}-2x \right)^n$
Коэффициент третьего элемента равен 105
Найти двенадцатый элемент
$C_{n}^2=105=\frac{n!}{2!(n-2)!}\quad n=15$
$C^{11}_{15}=\frac{15!}{11!4!}=105\cdot13=1365$
$a_{12}=1365\cdot \left( \frac{1}{\sqrt{ 3x }} \right)^4\cdot (-2x)^{11}=-\frac{931840x^9}{3}$

$C_{16}^{n-1}z^n\left( \frac{1}{z^3} \right)^{16-n}=\frac{16!}{(n-1)!(17-n)!}\cdot z^n\cdot\left( \frac{1}{z^3} \right)^{16}\cdot z^{3n}$

$(x+y+z)^3=C^0_{3}(x+y)^3+C^1_{3}(x+y)^2z+C_{3}^2(x+y)z^2+C^3_{3}z^3=$
$=x^3+3x^2y+3xy^2+y^3+3(x^2+2xyz+y^2z)+3(z^2x+yz^2)+z^3$




$(x+y+z)^9 = \sum\limits_{i=0}^9C^i_{9}(x+y)^{9-i}\cdot z^i$

Подробная запись:

$$
\begin{aligned}
(x+y+z)^9 = &\ x^9 + y^9 + z^9 \\
          + &\ 9\,(x^8y + x^8z + xy^8 + xz^8 + y^8z + yz^8) \\
          + &\ 36\,(x^7y^2 + x^7z^2 + x^2y^7 + x^2z^7 + y^7z^2 + y^2z^7) \\
          + &\ 84\,(x^7yz + xy^7z + xyz^7) \\
          + &\ 126\,(x^6y^3 + x^6z^3 + x^3y^6 + x^3z^6 + y^6z^3 + y^3z^6) \\
          + &\ 252\,(x^6y^2z + x^6yz^2 + x^2y^6z + x^2yz^6 + xy^6z^2 + xy^2z^6) \\
          + &\ 504\,(x^5y^4 + x^5z^4 + x^4y^5 + x^4z^5 + y^5z^4 + y^4z^5) \\
          + &\ 630\,(x^5y^3z + x^5yz^3 + x^3y^5z + x^3yz^5 + xy^5z^3 + xy^3z^5) \\
          + &\ 756\,(x^5y^2z^2 + x^2y^5z^2 + x^2y^2z^5) \\
          + &\ 1260\,(x^4y^3z^2 + x^4y^2z^3 + x^3y^4z^2 + x^3y^2z^4 + x^2y^4z^3 + x^2y^3z^4) \\
          + &\ 1680\,x^3y^3z^3
\end{aligned}
$$

